Generalize retry loop proof to allow default value
Previously, the fueled retry always ran the program at least once. More
general result shows that even if the fueled retry returns any result
when given insufficient fuel, the coinductive retry is equivalent. This
is easier to use since it means the inductive proof of fueled retry gets
the base case for free (it just returns some failure value) and only has
to reason about the inductive case.

src/RetryLoop.v
@@ -7,14 +7,14 @@ Section RetryLoop.
   Context {St:StateTypes}.
   Variable G:Protocol St.
 
-  Fixpoint retry_n {T P Q} (guard: forall (v:T), {P v}+{Q v}) (p: @cprog St T) n :=
+  Fixpoint retry_n {T P Q} (guard: forall (v:T), {P v}+{Q v}) (v0: T) (p: @cprog St T) n :=
     match n with
-    | 0 => p
+    | 0 => Ret v0
     | S n' => v <- p;
                if guard v then
                  Ret v
                else
-                 retry_n guard p n'
+                 retry_n guard v0 p n'
     end.
 
   CoFixpoint retry {T P Q} (guard: forall (v:T), {P v}+{Q v}) (p: @cprog St T) :=
@@ -54,7 +54,7 @@ Section RetryLoop.
 
   Theorem retry_exec : forall T P Q (guard: forall (v:T), {P v}+{Q v}) p,
       forall tid st out, exec G tid st (retry guard p) out ->
-                    (exists n, exec G tid st (retry_n guard p n) out) /\
+                    (exists n, forall v0, exec G tid st (retry_n guard v0 p n) out) /\
                     match out with
                     | Finished _ _ v => exists H, guard v = left H
                     | Error => True
@@ -71,21 +71,25 @@ Section RetryLoop.
     - case_eq (guard v); intros; replace (guard v) in *.
       + CCLTactics.inv_ret.
         intuition eauto.
-        exists 0; simpl; eauto.
+        exists 1; intros; simpl.
+        eapply ExecBindFinish; eauto.
+        replace (guard v).
+        eapply ExecRet; eauto.
       + rewrite retry_unfold in IHexec2.
         specialize (IHexec2 _ _ guard p); intuition.
         deex.
-        exists (S n); simpl.
+        exists (S n); intros; simpl.
         eapply ExecBindFinish; eauto.
         simpl_match; eauto.
     - inversion Heqc; repeat inj_pair2.
       intuition.
-      exists 0; eauto.
+      exists 1; simpl; intros.
+      eapply ExecBindFail; eauto.
   Qed.
 
-  Theorem retry_triple : forall T P Q (guard: forall (v:T), {P v}+{Q v}) p
+  Theorem retry_triple : forall T P Q (guard: forall (v:T), {P v}+{Q v}) v0 p
                          A (spec: Spec A T) tid,
-      (forall n, cprog_triple G tid spec (retry_n guard p n)) ->
+      (forall n, cprog_triple G tid spec (retry_n guard v0 p n)) ->
       cprog_triple G tid (fun a st =>
                             {| precondition := precondition (spec a st);
                                postcondition :=
@@ -96,24 +100,26 @@ Section RetryLoop.
   Proof.
     unfold cprog_triple; intros; simpl in *.
     apply retry_exec in H1; intuition; repeat deex.
+    specialize (H1 v0).
     eapply H in H1; eauto.
     destruct out; intuition eauto.
   Qed.
 
-  Theorem retry_triple' : forall T P Q (guard: forall (v:T), {P v}+{Q v}) p
+  Theorem retry_triple' : forall T P Q (guard: forall (v:T), {P v}+{Q v}) v0 p
                          A (spec: Spec A T) tid,
-      (forall n, cprog_triple G tid spec (retry_n guard p n)) ->
+      (forall n, cprog_triple G tid spec (retry_n guard v0 p n)) ->
       cprog_triple G tid spec (retry guard p).
   Proof.
     intros.
     unfold cprog_triple; intros; simpl in *.
     apply retry_exec in H1; intuition; repeat deex.
+    specialize (H1 v0).
     eapply H in H1; eauto.
   Qed.
 
-  Corollary retry_spec : forall T P Q (guard: forall (v:T), {P v}+{Q v}) p
+  Corollary retry_spec : forall T P Q (guard: forall (v:T), {P v}+{Q v}) v0 p
                          A (spec: Spec A T) tid,
-      (forall n, cprog_spec G tid spec (retry_n guard p n)) ->
+      (forall n, cprog_spec G tid spec (retry_n guard v0 p n)) ->
       cprog_spec G tid (fun a st =>
                             {| precondition := precondition (spec a st);
                                postcondition :=
@@ -124,20 +130,20 @@ Section RetryLoop.
   Proof.
     intros.
     apply triple_spec_equiv.
-    apply retry_triple; intros.
+    eapply retry_triple; intros.
     apply triple_spec_equiv.
     auto.
   Qed.
 
-  Corollary retry_spec' : forall T P Q (guard: forall (v:T), {P v}+{Q v}) p
+  Corollary retry_spec' : forall T P Q (guard: forall (v:T), {P v}+{Q v}) v0 p
                          A (spec: Spec A T) tid,
-      (forall n, cprog_spec G tid spec (retry_n guard p n)) ->
+      (forall n, cprog_spec G tid spec (retry_n guard v0 p n)) ->
       cprog_spec G tid spec (retry guard p).
   Proof.
     intros.
     intros.
     apply triple_spec_equiv.
-    apply retry_triple'; intros.
+    eapply retry_triple'; intros.
     apply triple_spec_equiv.
     auto.
   Qed.
